Launchbury/Abstract-Denotational-Props.thy
@@ -150,7 +150,7 @@ qed
 
 lemma fmap_restr_monofun_relaxed:
   "op f!\<^sub>\<bottom> \<rho> \<sqsubseteq> op f!\<^sub>\<bottom>\<rho>' \<Longrightarrow> op f!\<^sub>\<bottom> (\<rho> f|` S) \<sqsubseteq> op f!\<^sub>\<bottom> (\<rho>' f|` S)"
-by (auto simp add: below_fun_def lookup_fmap_restr_eq)
+by (auto simp add: below_fun_def fmap_lookup_bot_fmap_restr_eq)
 
 lemma HSem_monofun_relaxed':
   assumes "\<And>x \<rho> \<rho>'. x \<in> heapVars h \<Longrightarrow> op f!\<^sub>\<bottom> \<rho> \<sqsubseteq> op f!\<^sub>\<bottom>\<rho>' \<Longrightarrow> \<lbrakk> the (map_of h x) \<rbrakk>\<^bsub>\<rho>\<^esub> \<sqsubseteq> \<lbrakk> the (map_of h x) \<rbrakk>\<^bsub>\<rho>'\<^esub>"
